robochart/untimed/Actions.thy
@@ -50,7 +50,7 @@ lift_definition
   is "SpecC"
   by (simp add: closure)
 
-utp_lift_notation spec (1 2)
+utp_lift_notation spec (0)
 
 lift_definition assumption :: "'s upred \<Rightarrow> ('s, 'e) Action" ("[_]\<^sub>A") is "AssumeCircus"
   by (simp add: closure)
@@ -65,7 +65,7 @@ lift_definition cond :: "'s upred \<Rightarrow> ('s, 'e) Action \<Rightarrow> ('
   ("if _ then _ else _ end")
   is "\<lambda> b P Q. cond_srea P b Q" by (simp add: closure)
 
-utp_lift_notation cond (0)
+utp_lift_notation cond (1 2)
 
 lift_definition assigns :: "'s usubst \<Rightarrow> ('s, 'e) Action" is "AssignsCSP"
   by (simp_all add: closure)
@@ -95,14 +95,14 @@ adhoc_overloading usubst asubst
 lift_definition guard :: "'s upred \<Rightarrow> ('s, 'e) Action \<Rightarrow> ('s, 'e) Action" (infixr "\<^bold>&" 60) is "GuardCSP"
   by (simp add: closure)
 
-utp_lift_notation guard (0)
+utp_lift_notation guard (1)
 
 lift_definition sync :: "'e \<Rightarrow> ('s, 'e) Action" ("\<^bold>s'(_')") is "\<lambda> e. e \<^bold>\<rightarrow> Skip" by (simp add: closure)
 
 lift_definition send :: "('a \<Rightarrow> 'e) \<Rightarrow> ('a, 's) uexpr \<Rightarrow> ('s, 'e) Action" ("_\<^bold>!'(_')" [999,0] 999)
   is "\<lambda> c v. c!(v) \<^bold>\<rightarrow> Skip" by (simp add: closure)
 
-utp_lift_notation send (1)
+utp_lift_notation send (0)
 
 lift_definition receive :: "('a \<Rightarrow> 'e) \<Rightarrow> ('a \<Longrightarrow> 's) \<Rightarrow> ('s, 'e) Action" ("_\<^bold>?'(_')" [999,0] 999)
   is "\<lambda> c x. c?(v) \<^bold>\<rightarrow> x :=\<^sub>C \<guillemotleft>v\<guillemotright>" by (simp add: InputCSP_def closure)
